src/Implementations/Transaction/Transaction.v
@@ -1,40 +1,37 @@
-Require Import Compare_dec Framework FSParameters TransactionCacheLayer.
+Require Import Compare_dec Lia Framework TotalMem FSParameters TransactionCacheLayer.
 
-Fixpoint get_latest (txn: list (addr * value)) a :=
+Fixpoint get_first (txn: list (addr * value)) a :=
   match txn  with
   | ad :: txn' =>
     if addr_eq_dec a (fst ad) then
       Some (snd ad)
     else
-      get_latest txn' a
+      get_first txn' a
   | [] =>
     None
   end.
-
-Definition start :=
-  _ <- |TCCO| Delete _;
-  Ret tt.
-
-(** Reverses before submitting **)
-Definition commit :=
-  txn <- |TCCO| Get _;
-  let al := map fst (rev txn) in
-  let vl := map snd (rev txn) in
-  let dedup_al := dedup_last addr_dec al in
-  let dedup_vl := dedup_by_list addr_dec al vl in
-  _ <- |TCDO| Write dedup_al dedup_vl;
-  _ <- |TCCO| Delete _;
-  Ret tt.
 
 Definition abort :=
   _ <- |TCCO| Delete _;
   Ret tt.
 
+Definition commit :=
+  txn <- |TCCO| Get _;
+  let al := map fst txn in
+  let vl := map snd txn in
+  let dedup_al := dedup_last addr_dec (rev al) in
+  let dedup_vl := dedup_by_list addr_dec (rev al) (rev vl) in
+  _ <- |TCDO| Write dedup_al dedup_vl;
+  _ <- |TCCO| Delete _;
+  Ret tt.
+
+(* Definition abort := start. *)
+
 (* if you read out of bounds, you get 0 block *)
 Definition read a :=
   if lt_dec a data_length then
     txn <- |TCCO| Get _;
-    match get_latest txn a with
+    match get_first txn a with
     | Some v =>
       Ret v
     | None =>
@@ -60,11 +57,256 @@ Definition recover :=
   _ <- |TCDO| Recover;
   Ret tt.
 
-Definition transaction_rep (tcd: TransactionCacheLang.(state)) (td: (@mem addr addr_dec value) * (@total_mem addr addr_dec value)):=
+Definition transaction_rep (tcd: TransactionCacheLang.(state)) (td: (@total_mem addr addr_dec value) * (@total_mem addr addr_dec value)):=
   let al := map fst (fst tcd) in
   let vl := map snd (fst tcd) in
-  let dedup_al := dedup_last addr_dec al in
-  let dedup_vl := dedup_by_list addr_dec al vl in
-  fst td = Mem.upd_batch empty_mem dedup_al dedup_vl /\
+  fst td = upd_batch (snd tcd) (rev al) (rev vl) /\
   snd td = snd tcd.
   
+
+Definition transaction_reboot_rep (tcd: TransactionCacheLang.(state)) (td: (@total_mem addr addr_dec value) * (@total_mem addr addr_dec value)):=
+  fst tcd = [] /\
+  snd td = snd tcd.
+
+Theorem abort_finished:
+  forall u s o s' r,
+    exec TransactionCacheLang u o s abort (Finished s' r) ->
+    fst s' = [] /\ snd s' = snd s.
+Proof.
+  unfold abort; intros; repeat invert_exec; eauto.
+Qed.
+
+Theorem abort_crashed:
+  forall u s o s',
+    exec TransactionCacheLang u o s abort (Crashed s') ->
+    snd s' = snd s.
+Proof.
+  unfold abort; intros; repeat invert_exec; eauto.
+  split_ors; cleanup; repeat invert_exec; eauto.
+Qed.
+
+(*
+Definition abort_finished := start_finished.
+Definition abort_crashed := start_crashed.
+ *)
+
+Lemma upd_batch_dedup_last_dedup_by_list:
+  forall A AEQ V l_a l_v (tm: @total_mem A AEQ V),
+    length l_a = length l_v ->
+    upd_batch tm l_a l_v =
+    upd_batch tm (dedup_last AEQ l_a) (dedup_by_list AEQ l_a l_v).
+Proof.
+  induction l_a; simpl; intros; eauto.
+  destruct l_v; simpl in *; try congruence; eauto.
+  destruct (in_dec AEQ a l_a).
+  rewrite upd_batch_upd_in_noop; eauto.
+  simpl; eauto.
+Qed.
+
+Set Nested Proofs Allowed.
+
+Theorem commit_finished :
+  forall u s o s' r td,
+    transaction_rep s td ->
+    exec TransactionCacheLang u o s commit (Finished s' r) ->
+    transaction_rep s' (fst td, fst td) \/
+    transaction_rep s' (snd td, snd td).
+Proof.
+  unfold commit, transaction_rep; simpl; intros.
+  repeat invert_exec; simpl in *; cleanup;
+  repeat cleanup_pairs.
+  {
+    left; simpl; split;
+    apply upd_batch_dedup_last_dedup_by_list; eauto;
+    repeat rewrite rev_length, map_length; eauto.    
+  }
+  right; eauto.
+Qed.
+
+Theorem commit_crashed :
+  forall u s o s' td,
+    transaction_rep s td ->
+    exec TransactionCacheLang u o s commit (Crashed s') ->
+    snd s' = snd td \/ snd s' = fst td.
+Proof.
+  unfold commit, transaction_rep; simpl; intros.
+  repeat invert_exec; simpl in *; cleanup;
+  repeat cleanup_pairs.
+  repeat (match goal with
+    [H: exec _ _ _ _ _ _ \/ _ |- _] =>
+    destruct H
+  end; cleanup; simpl in *;
+  repeat invert_exec; simpl in *;
+  try solve [ left; eauto ];
+  try solve [
+    right; setoid_rewrite upd_batch_dedup_last_dedup_by_list at 2; eauto;
+    repeat rewrite rev_length, map_length; eauto ]).
+Qed.
+
+Lemma get_first_some_upd_batch:
+  forall l tm a v,
+    get_first l a = Some v ->
+    upd_batch tm (rev (map fst l)) (rev (map snd l)) a = v.
+Proof.
+  induction l; simpl; intros; try congruence.
+  rewrite upd_batch_app; simpl.
+  cleanup.
+  rewrite upd_eq; eauto.
+  rewrite upd_ne; eauto.
+  repeat rewrite rev_length, map_length; eauto.
+Qed.
+
+Lemma get_first_none_not_in:
+  forall l a,
+    get_first l a = None ->
+    ~In a (map fst l).
+Proof.
+  induction l; simpl in *; intuition.
+  simpl in *; cleanup; try congruence.
+  simpl in *; destruct (addr_eq_dec a a0);
+  try congruence; eauto.
+Qed.
+
+Definition read_finished :
+  forall u s o s' r td a,
+    transaction_rep s td ->
+    exec TransactionCacheLang u o s (read a) (Finished s' r) ->
+    transaction_rep s' td /\
+    ((a < data_length /\ r = (fst td) a) \/
+     (a >= data_length /\ r = value0)).
+Proof.
+  unfold read, transaction_rep; intros; cleanup;
+  repeat invert_exec; cleanup;
+  repeat cleanup_pairs; split; eauto.
+  {
+    left; split; eauto.
+    erewrite get_first_some_upd_batch; eauto.
+  }
+  {
+    left; split; eauto.
+    rewrite upd_batch_ne; eauto.
+
+    intros Hx.
+    apply in_rev in Hx; eauto.
+    apply get_first_none_not_in in Hx; eauto.
+  }
+  {
+    right; split; eauto; lia.
+  }
+Qed.
+
+Definition read_crashed :
+  forall u s o s' td a,
+    transaction_rep s td ->
+    exec TransactionCacheLang u o s (read a) (Crashed s') ->
+    transaction_rep s' td.
+Proof.
+  unfold read, transaction_rep; simpl; intros.
+  cleanup; repeat invert_exec; simpl in *; cleanup;
+  repeat cleanup_pairs;
+  repeat (
+      match goal with
+    [H: exec _ _ _ _ _ _ \/ _ |- _] =>
+    destruct H
+  end; cleanup; simpl in *;
+      repeat invert_exec; cleanup;
+      simpl in *; eauto).
+  invert_exec; simpl; eauto.
+  invert_exec; simpl; eauto.
+  repeat (
+      match goal with
+    [H: exec _ _ _ _ _ _ \/ _ |- _] =>
+    destruct H
+  end; cleanup; simpl in *;
+      repeat invert_exec; cleanup;
+      simpl in *; eauto).
+  eauto.
+Qed.
+
+
+Definition write_finished :
+  forall u s o s' r td a v,
+    transaction_rep s td ->
+    exec TransactionCacheLang u o s (write a v) (Finished s' r) ->
+    (a < data_length /\
+     length (fst s) < log_length /\
+     transaction_rep s' (upd (fst td) a v, snd td)) \/
+    ((a >= data_length \/
+      length (fst s) >= log_length) /\
+     transaction_rep s' td).
+Proof.
+  unfold write, transaction_rep; intros; cleanup;
+  repeat invert_exec; cleanup; simpl in *;
+  repeat cleanup_pairs; eauto.
+  {
+    left; split; eauto.
+    erewrite upd_batch_app; simpl; eauto.
+    repeat rewrite rev_length, map_length; eauto.
+  }
+  {
+    right; split; eauto; lia.
+  }
+  {
+    right; split; eauto; lia.
+  }
+Qed.
+
+Definition write_crashed :
+  forall u s o s' td a v,
+    transaction_rep s td ->
+    exec TransactionCacheLang u o s (write a v) (Crashed s') ->
+    transaction_rep s' (upd (fst td) a v, snd td) \/
+    transaction_rep s' td.
+Proof.
+  unfold write, transaction_rep; simpl; intros.
+  cleanup; repeat invert_exec; simpl in *; cleanup;
+  repeat cleanup_pairs;
+  repeat (
+      match goal with
+    [H: exec _ _ _ _ _ _ \/ _ |- _] =>
+    destruct H
+  end; cleanup; simpl in *;
+      repeat invert_exec; cleanup;
+      simpl in *; eauto).
+  invert_exec; simpl; eauto.
+  repeat (
+      match goal with
+    [H: exec _ _ _ _ _ _ \/ _ |- _] =>
+    destruct H
+  end; cleanup; simpl in *;
+      repeat invert_exec; cleanup;
+      simpl in *; eauto).
+  {
+    left; split; eauto.
+    erewrite upd_batch_app; simpl; eauto.
+    repeat rewrite rev_length, map_length; eauto.
+  }
+  {
+    invert_exec.
+    right; split; eauto; lia.
+  }
+  {
+    right; split; eauto; lia.
+  }
+Qed.
+
+Definition recover_finished :
+  forall u s o s' r td,
+    transaction_reboot_rep s td ->
+    exec TransactionCacheLang u o s recover (Finished s' r) ->
+    transaction_rep s' (snd td, snd td).
+Proof.
+  unfold recover, transaction_reboot_rep, transaction_rep; intros.
+  repeat invert_exec; cleanup; repeat cleanup_pairs; simpl; eauto.
+Qed.
+
+Definition recover_crashed :
+  forall u s o s' td,
+    transaction_reboot_rep s td ->
+    exec TransactionCacheLang u o s recover (Crashed s') ->
+    snd s' = snd s.
+Proof.
+  unfold recover, transaction_reboot_rep, transaction_rep; intros.
+  repeat invert_exec; cleanup; repeat cleanup_pairs; simpl; eauto.
+  split_ors; cleanup; repeat invert_exec; eauto.
+Qed.
