src/Layers/BasicLayers/Crypto/CryptoLayer.v
@@ -1,5 +1,6 @@
 Require Import Framework.
 Import ListNotations.
+Import Mem.
 
 Set Implicit Arguments.
 
@@ -7,13 +8,14 @@ Instance value_eq_dec: EqDec value := value_dec.
 Instance hash_eq_dec: EqDec hash := hash_dec.
 
 Definition hashmap := @mem hash hash_dec (hash * value).
-  
+Definition encryption_map:= @mem value value_dec (key * value).
+
   Inductive token' :=
   | Key : key -> token'
   | Crash : token'
   | Cont : token'.
 
-  Definition state' := (list key * hashmap)%type.
+  Definition state' := (list key * hashmap * encryption_map)%type.
 
   Inductive crypto_prog : Type -> Type :=
   | GetKey : crypto_prog key
@@ -26,26 +28,36 @@ Definition hashmap := @mem hash hash_dec (hash * value).
 
   | ExecHash : 
       forall s h v u,
-        let kl := fst s in
-        let hm := snd s in
+        let kl := fst (fst s) in
+        let hm := snd (fst s) in
+        let em := snd s in
         let hv := hash_function h v in
         consistent hm hv (h, v) ->
-        exec' u Cont s (Hash h v) (Finished (kl, (upd hm hv (h, v))) hv)
+        exec' u Cont s (Hash h v) (Finished (kl, (upd hm hv (h, v)), em) hv)
              
   | ExecEncrypt : 
       forall s k v u,
-        exec' u Cont s (Encrypt k v) (Finished s (encrypt k v))
+        let kl := fst (fst s) in
+        let hm := snd (fst s) in
+        let em := snd s in
+        consistent em (encrypt k v) (k, v) -> 
+        exec' u Cont s (Encrypt k v) (Finished (kl, hm, upd em (encrypt k v) (k, v)) (encrypt k v))
 
   | ExecDecrypt : 
       forall s ev k u,
-        exec' u Cont s (Decrypt k ev) (Finished s (decrypt k ev))
+        let kl := fst (fst s) in
+        let hm := snd (fst s) in
+        let em := snd s in
+        consistent em ev (k, decrypt k ev) ->
+        exec' u Cont s (Decrypt k ev) (Finished (kl, hm, upd em ev (k, decrypt k ev)) (decrypt k ev))
 
   | ExecGetKey : 
       forall s k u,
-        let kl := fst s in
-        let hm := snd s in
+        let kl := fst (fst s) in
+        let hm := snd (fst s) in
+        let em := snd s in
         ~In k kl ->
-        exec' u (Key k) s GetKey (Finished ((k::kl), hm) k)
+        exec' u (Key k) s GetKey (Finished ((k::kl), hm, em) k)
  
   | ExecCrash :
       forall T d (p: crypto_prog T) u,
@@ -75,7 +87,3 @@ Definition hashmap := @mem hash hash_dec (hash * value).
       exec_deterministic_wrt_token'.
   
   Definition CryptoLang := Build_Language CryptoOperation.
-
-Notation "| p |" := (Op CryptoOperation p)(at level 60).
-Notation "x <-| p1 ; p2" := (Bind (Op CryptoOperation p1) (fun x => p2))(right associativity, at level 60).
-Notation "p >> s" := (p s) (right associativity, at level 60, only parsing).
