src/Implementations/LogCache/LogCache.v
@@ -153,583 +153,7 @@ Definition cached_log_reboot_rep merged_disk (s: Language.state CachedDiskLang) 
 
 Set Nested Proofs Allowed.
 
-(*** LEMMAS ***)
-  Lemma upd_batch_noop:
-    forall A (AEQ: EqDec A) V (l_a: list A) (l_v: list V) m tm,
-      Mem.upd_batch m l_a l_v = m ->
-      Forall (fun a => m a = None) l_a -> 
-      length l_a = length l_v ->
-      upd_batch tm l_a l_v = tm.
-  Proof.
-    induction l_a; simpl; intros; eauto.
-    destruct l_v; eauto.
-    inversion H0; cleanup.
-    destruct (in_dec AEQ a l_a).
-    {
-      rewrite Mem.upd_batch_upd_in_noop in H; eauto.
-      rewrite upd_batch_upd_in_noop; eauto.
-    }
-    {
-      rewrite Mem.upd_batch_upd in H; eauto.
-      eapply equal_f with (x:= a) in H.              
-      rewrite Mem.upd_eq in *; eauto; cleanup.
-    }
-  Qed.
-
-  Lemma list_upd_batch_noop:
-    forall A (AEQ: EqDec A) V (l_l_a: list (list A)) (l_l_v: list (list V)) m,
-      Mem.list_upd_batch m l_l_a l_l_v = m ->
-      Forall (Forall (fun a => m a = None)) l_l_a ->
-      Forall2 (fun l_a l_v => length l_a = length l_v) l_l_a l_l_v ->
-      (forall tm, list_upd_batch tm l_l_a l_l_v = tm).
-  Proof.
-    do 4 intro.
-    eapply rev_ind with
-        (P:= fun l_l_a =>
-               forall (l_l_v : list (list V)) (m : mem),
-                 Mem.list_upd_batch m l_l_a l_l_v = m ->
-                 Forall (Forall (fun a : A => m a = None)) l_l_a ->                      
-                 Forall2 (fun l_a l_v => length l_a = length l_v) l_l_a l_l_v ->
-                 forall tm : total_mem, list_upd_batch tm l_l_a l_l_v = tm);
-    simpl; intros; eauto.
-    {
-      destruct (nil_or_app l_l_v); cleanup.
-      destruct (l++[x]); simpl; eauto.
-      
-      
-      eapply_fresh forall2_length in H2.
-      repeat rewrite app_length in *; simpl in *.
-      eapply_fresh Forall2_app_split in H2; cleanup; eauto; try lia.
-      eapply_fresh forall_app_l in H1.
-      eapply_fresh forall_app_r in H1.
-      rewrite Mem.list_upd_batch_app in H0; simpl in *; try lia.
-      inversion Hx0; cleanup.
-      rewrite list_upd_batch_app; simpl in *; try lia.
-      destruct (nil_or_app x); cleanup;
-      simpl in *; eauto.
-      destruct (nil_or_app x0); cleanup.
-      destruct (x3 ++ [x2]); simpl in *; eauto.
-      inversion H4; cleanup.
-      repeat rewrite app_length in *; simpl in *.
-      rewrite Mem.upd_batch_app in *; simpl in *; try lia.
-      apply forall_app_l in H7; inversion H7; cleanup.
-      apply equal_f with (x0:= x2) in H0.
-      rewrite Mem.upd_eq in *; eauto; cleanup.
-    }
-  Qed.
-
-  Lemma upd_batch_noop_empty_mem:
-    forall A (AEQ: EqDec A) V (l_a: list A) (l_v: list V) tm,
-      Mem.upd_batch empty_mem l_a l_v = empty_mem ->
-      length l_a = length l_v ->
-      upd_batch tm l_a l_v = tm.
-  Proof.
-    induction l_a; simpl; intros; eauto.
-    destruct l_v; eauto.
-    destruct (in_dec AEQ a l_a).
-    {
-      rewrite Mem.upd_batch_upd_in_noop in H; eauto.
-      rewrite upd_batch_upd_in_noop; eauto.
-    }
-    {
-      rewrite Mem.upd_batch_upd in H; eauto.
-      eapply equal_f with (x:= a) in H.              
-      rewrite Mem.upd_eq in *; eauto.
-      unfold empty_mem in *; congruence.
-    }
-  Qed.
-  
-  Lemma upd_batch_eq_empty_mem:
-    forall A (AEQ: EqDec A) V (l_a: list A) (l_v: list V) m,
-      Mem.upd_batch m l_a l_v = empty_mem ->
-      m = empty_mem /\
-      (l_a = [] \/ l_v = []).
-  Proof.
-    induction l_a; simpl; intros; eauto.
-    destruct l_v; eauto.
-    eapply IHl_a in H.
-    destruct H.
-    eapply equal_f with (x:=a) in H.
-    rewrite Mem.upd_eq in H; eauto.
-    unfold empty_mem in *; congruence.
-  Qed.
-
-  Lemma list_upd_batch_eq_empty_mem:
-    forall A (AEQ: EqDec A) V (l_l_a: list (list A)) (l_l_v: list (list V)) m,
-      Mem.list_upd_batch m l_l_a l_l_v = empty_mem ->
-      m = empty_mem /\
-      (forall tm, list_upd_batch tm l_l_a l_l_v = tm).
-  Proof.
-    induction l_l_a; simpl; intros; eauto.
-    destruct l_l_v; eauto.
-    eapply IHl_l_a in H.
-    destruct H.
-    apply upd_batch_eq_empty_mem in H.
-    destruct H.
-    split; eauto.
-    intros; rewrite H0.            
-    intuition; subst; simpl; eauto.
-    destruct a; eauto.
-  Qed.
-
-  Lemma skipn_eq_nil:
-    forall T (l: list T) n,
-      skipn n l = nil ->
-      l = [] \/ n >= length l.
-  Proof.
-    induction l; simpl; intros; eauto.
-    destruct n; simpl in *; eauto.
-    apply IHl in H.
-    intuition subst; simpl; try lia.
-  Qed.
-
-  Fixpoint remove_by_fst {A} {AEQ: EqDec A} {V} (a: A) (l_av: list (A * V)) :=
-    match l_av with
-    | nil => nil
-    | av :: l_av' =>
-      if (AEQ a (fst av)) then
-        remove_by_fst a l_av'
-      else
-        av :: remove_by_fst a l_av'
-    end.
-
-  Lemma remove_by_fst_not_in:
-    forall A (AEQ: EqDec A) V (l: list (A * V)) a,
-      ~ In a (map fst (remove_by_fst a l)).
-  Proof.
-    induction l; simpl; eauto.
-    intros.
-    destruct (AEQ a0 (fst a)); subst; eauto.
-    simpl; intuition eauto.
-  Qed.
-
-  Lemma remove_by_fst_incl:
-    forall A (AEQ: EqDec A) V (l: list (A * V)) a,
-      incl (remove_by_fst a l) l.
-  Proof.
-    unfold incl; induction l; simpl; intros; eauto.
-    destruct (AEQ a0 (fst a)); subst; eauto.
-    inversion H; simpl in *; intuition eauto.
-  Qed.
-  
-  Lemma upd_batch_upd_remove_by_fst:
-    forall A AEQ V l_a l_v (m: @mem A AEQ V) a v,
-    let l_av := remove_by_fst a (combine l_a l_v) in
-      Mem.upd (Mem.upd_batch m l_a l_v) a v =
-      Mem.upd (Mem.upd_batch m (map fst l_av) (map snd l_av)) a v.
-  Proof.
-    unfold incl; induction l_a; simpl; intros; eauto.
-    {
-      destruct l_v; simpl; eauto.
-      destruct (AEQ a0 a); subst.
-      rewrite IHl_a.
-      rewrite Mem.upd_batch_upd; eauto.
-      rewrite Mem.upd_repeat; eauto.
-      apply remove_by_fst_not_in.
-
-      rewrite IHl_a; simpl; intuition eauto.
-    }
-  Qed.
-
-   Lemma upd_batch_upd_remove_by_fst_total:
-    forall A AEQ V l_a l_v (m: @total_mem A AEQ V) a v,
-    let l_av := remove_by_fst a (combine l_a l_v) in
-      upd (upd_batch m l_a l_v) a v =
-      upd (upd_batch m (map fst l_av) (map snd l_av)) a v.
-  Proof.
-    unfold incl; induction l_a; simpl; intros; eauto.
-    {
-      destruct l_v; simpl; eauto.
-      destruct (AEQ a0 a); subst.
-      rewrite IHl_a.
-      rewrite upd_batch_upd; eauto.
-      rewrite upd_repeat; eauto.
-      apply remove_by_fst_not_in.
-
-      rewrite IHl_a; simpl; intuition eauto.
-    }
-  Qed.
-
-  Lemma upd_batch_dedup_by_fst:
-    forall A AEQ V l_a l_v (m: @mem A AEQ V),
-    let l_av := dedup_by_fst AEQ (combine l_a l_v) in
-    length l_a = length l_v ->
-    Mem.upd_batch m l_a l_v =
-    Mem.upd_batch m (map fst l_av) (map snd l_av).
-  Proof.
-    induction l_a; simpl; intros; eauto.
-    {
-      destruct l_v; simpl; eauto.
-      rewrite map_fst_combine.
-      destruct (in_dec AEQ a l_a); subst.
-      rewrite Mem.upd_batch_upd_in_noop; eauto.
-      simpl; eauto.
-      simpl in *; lia.
-    }
-  Qed.
-
-  Lemma upd_batch_dedup_by_fst_total:
-    forall A AEQ V l_a l_v (m: @total_mem A AEQ V),
-    let l_av := dedup_by_fst AEQ (combine l_a l_v) in
-    length l_a = length l_v ->
-    upd_batch m l_a l_v =
-    upd_batch m (map fst l_av) (map snd l_av).
-  Proof.
-    induction l_a; simpl; intros; eauto.
-    {
-      destruct l_v; simpl; eauto.
-      rewrite map_fst_combine.
-      destruct (in_dec AEQ a l_a); subst.
-      rewrite upd_batch_upd_in_noop; eauto.
-      simpl; eauto.
-      simpl in *; lia.
-    }
-  Qed.
-
-  Fixpoint flatten {A} (l_l_a: list (list A)) :=
-    match l_l_a with
-    | nil => nil
-    | l_a :: l_l_a' =>
-      l_a ++ flatten l_l_a'
-    end.
-
-  Lemma flatten_app:
-    forall A (l1 l2: list (list A)),
-      flatten (l1 ++ l2) = flatten l1 ++ flatten l2.
-  Proof.
-    induction l1; simpl; intros; eauto.
-    rewrite <- app_assoc; eauto.
-    rewrite IHl1; eauto.
-  Qed.
-
-  Lemma flatten_length_eq:
-    forall A V l1 l2,
-      Forall2 (fun (l_a0 : list A) (l_v0 : list V) => length l_a0 = length l_v0) l1 l2 ->
-      length (flatten l1) = length (flatten l2).
-  Proof.
-    induction l1; simpl; intros; eauto.
-    apply forall2_length in H; destruct l2; simpl in *; lia.
-    eapply_fresh forall2_length in H; destruct l2; simpl in *; try lia.
-    inversion H; cleanup.
-    repeat rewrite app_length.
-    erewrite IHl1; eauto; lia.
-  Qed.
-
-  Lemma list_upd_batch_to_upd_batch:
-    forall A AEQ V l_a l_v (m: @mem A AEQ V),
-    Forall2 (fun l_a l_v => length l_a = length l_v) l_a l_v ->
-    Mem.list_upd_batch m l_a l_v =
-    Mem.upd_batch m (flatten l_a) (flatten l_v).
-  Proof.
-    do 4 intro.
-    eapply rev_ind with
-        (P:= fun l_a =>
-        forall (l_v : list (list V)) (m : mem),
-  Forall2 (fun (l_a0 : list A) (l_v0 : list V) => length l_a0 = length l_v0) l_a l_v ->
-  Mem.list_upd_batch m l_a l_v = Mem.upd_batch m (flatten l_a) (flatten l_v));
-    simpl; intros; eauto.
-    {
-      eapply_fresh forall2_length in H0.
-      rewrite app_length in *; simpl in *.      
-      destruct (nil_or_app l_v); subst; simpl in *; try lia.
-      cleanup.
-      rewrite app_length in *; simpl in *.
-      eapply Forall2_app_split in H0; cleanup; try lia.
-      rewrite Mem.list_upd_batch_app; try lia.
-      simpl.
-      repeat rewrite flatten_app; simpl.
-      repeat rewrite app_nil_r.
-      rewrite Mem.upd_batch_app.
-      rewrite H; eauto; lia.
-      apply flatten_length_eq; eauto.
-    }
-  Qed.
-
-   Lemma list_upd_batch_to_upd_batch_total:
-    forall A AEQ V l_a l_v (m: @total_mem A AEQ V),
-    Forall2 (fun l_a l_v => length l_a = length l_v) l_a l_v ->
-    list_upd_batch m l_a l_v =
-    upd_batch m (flatten l_a) (flatten l_v).
-  Proof.
-    do 4 intro.
-    eapply rev_ind with
-        (P:= fun l_a =>
-        forall (l_v : list (list V)) (m : total_mem),
-  Forall2 (fun (l_a0 : list A) (l_v0 : list V) => length l_a0 = length l_v0) l_a l_v ->
-  list_upd_batch m l_a l_v = upd_batch m (flatten l_a) (flatten l_v));
-    simpl; intros; eauto.
-    {
-      eapply_fresh forall2_length in H0.
-      rewrite app_length in *; simpl in *.      
-      destruct (nil_or_app l_v); subst; simpl in *; try lia.
-      cleanup.
-      rewrite app_length in *; simpl in *.
-      eapply Forall2_app_split in H0; cleanup; try lia.
-      rewrite list_upd_batch_app; try lia.
-      simpl.
-      repeat rewrite flatten_app; simpl.
-      repeat rewrite app_nil_r.
-      rewrite upd_batch_app.
-      rewrite H; eauto; lia.
-      apply flatten_length_eq; eauto.
-    }
-  Qed.
-  
-  Lemma upd_batch_eq_upd_batch_total:
-    forall A AEQ V l_av1 l_av2 (tm: @total_mem A AEQ V) m,
-      let l_a1 := map fst l_av1 in
-      let l_a2 := map fst l_av2 in
-      let l_v1 := map snd l_av1 in
-      let l_v2 := map snd l_av2 in
-      
-      Mem.upd_batch m l_a1 l_v1 =
-      Mem.upd_batch m l_a2 l_v2 ->
-      Forall (fun a => m a = None) l_a1 ->
-      Forall (fun a => m a = None) l_a2 ->
-      NoDup l_a1 ->
-      NoDup l_a2 ->
-      upd_batch tm l_a1 l_v1 =
-      upd_batch tm l_a2 l_v2.
-  Proof.
-    induction l_av1; simpl; intros.
-    { (** l_av1 = [] **)
-      symmetry in H; eapply upd_batch_noop in H; eauto.
-      repeat rewrite map_length; eauto.
-    }
-    (** l_av1 = a::l **)
-    inversion H0; cleanup; clear H0.
-    inversion H2; cleanup; clear H2.
-    destruct l_av2; subst; simpl in *.
-    {(** l_a2 = [] **)
-      rewrite Mem.upd_batch_upd in *; eauto.
-      eapply equal_f with (x:= fst a) in H.
-      rewrite Mem.upd_eq in *; eauto; cleanup.
-    }
-    {(** l_a2 = a'::l' **)            
-      inversion H1; cleanup; clear H1.
-      inversion H3; cleanup; clear H3.
-      destruct a, p; simpl in *.
-      destruct (AEQ a a0); subst.
-      {(** a = a0 **)
-        assert_fresh (v = v0). {
-          apply equal_f with (x:= a0) in H.                
-          do 2 rewrite Mem.upd_batch_upd in *; eauto.
-          do 2 rewrite Mem.upd_eq in *; eauto; congruence.
-        }
-        subst.
-        eapply IHl_av1; eauto.
-        {
-          eapply Forall_forall; intros; intuition.
-          destruct (AEQ a0 x); subst; intuition.
-          rewrite Mem.upd_ne; eauto.
-          eapply Forall_forall in H7; eauto.
-        }
-        {
-          eapply Forall_forall; intros; intuition.
-          destruct (AEQ a0 x); subst; intuition.
-          rewrite Mem.upd_ne; eauto.
-          eapply Forall_forall in H9; eauto.
-        }
-      }
-      {(** a <> a0 **)
-        destruct (in_dec AEQ a (map fst l_av2)).
-        {(** In a (map fst l_av2) **)
-          eapply_fresh in_map_iff in i; cleanup.
-          eapply_fresh in_split in H1; eauto; cleanup.
-          repeat rewrite map_app in *; simpl in *.
-          rewrite Mem.upd_batch_app in H; eauto.
-          rewrite upd_batch_app.
-          simpl in *.
-          assert_fresh (v = snd x). {
-            do 2 rewrite Mem.upd_batch_upd in H; eauto.
-            apply equal_f with (x2:= fst x) in H.                
-            do 2 rewrite Mem.upd_eq in *; eauto; congruence.
-            intros Hx.
-            apply NoDup_app_r in H10; inversion H10; eauto.
-          }
-          subst.
-          rewrite <- Mem.upd_batch_upd in H; eauto.
-          rewrite Mem.upd_comm in H; eauto.
-          rewrite Mem.upd_to_upd_batch_singleton with (a:= a0) in H .
-          do 2 rewrite <- Mem.upd_batch_app in H; eauto.
-          replace ([a0] ++ map fst x0 ++ map fst x1)
-            with (map fst ((a0, v0) :: x0 ++ x1)) in H.
-          replace ([v0] ++ map snd x0 ++ map snd x1)
-            with (map snd ((a0, v0) :: x0 ++ x1)) in H.
-          eapply IHl_av1 in H; eauto.
-          rewrite H.
-          simpl.
-          rewrite <- upd_batch_upd; eauto.
-          rewrite upd_comm.
-          repeat rewrite map_app;
-          rewrite upd_batch_app; eauto.
-          all: try solve [repeat rewrite map_length; eauto].
-          all: try solve [simpl; repeat rewrite map_app; eauto].
-          {
-            eapply NoDup_remove_2 in H10.
-            intros Hx; apply H10.
-            apply in_app_iff; eauto.
-          }
-          {
-            eapply Forall_forall; intros.
-            eapply Forall_forall in H7; eauto.
-            destruct (AEQ x2 (fst x)); subst; intuition.
-            rewrite Mem.upd_ne; eauto.
-          }
-          {
-            simpl.
-            eapply NoDup_remove_2 in H10.
-            constructor; eauto.
-            rewrite Mem.upd_ne; eauto.
-            rewrite map_app; simpl.
-            apply Forall_forall; intros.
-            destruct (AEQ x2 (fst x)); subst; intuition.
-            rewrite Mem.upd_ne; eauto.
-            eapply Forall_forall in H9; eauto.
-            apply in_app_iff in H0.
-            apply in_app_iff; simpl; intuition eauto.
-          }
-          {
-            eapply NoDup_remove_1 in H10.
-            simpl; rewrite map_app; constructor; eauto.
-            
-            intros Hx; apply H2.
-            apply in_app_iff in Hx.
-            apply in_app_iff; simpl; intuition eauto.
-          }
-          {
-            eapply NoDup_remove_2 in H10.
-            intros Hx; apply H10.
-            apply in_app_iff; eauto.
-          }
-        }
-        {(** ~In a (map fst l_av2) **)
-          eapply equal_f with (x:= a) in H.
-          do 2 rewrite Mem.upd_batch_ne in H; eauto.
-          rewrite Mem.upd_eq in H; eauto.
-          rewrite Mem.upd_ne in H; eauto; cleanup.
-        }
-      }
-    }
-  Qed.
-
-  Lemma in_dedup_by_fst:
-      forall A AEQ B (l: list (A * B)) ab,
-        In ab (dedup_by_fst AEQ l) ->
-        In ab l.
-    Proof.
-      induction l; simpl; intros; eauto.
-      destruct (in_dec AEQ (fst a) (map fst l)); eauto.
-      inversion H; subst; eauto.
-    Qed.
-
-    
-    Lemma in_flatten:
-      forall A (l_l_a: list (list A)) a,
-        In a (flatten l_l_a) ->
-        exists l_a, In l_a l_l_a /\ In a l_a.
-    Proof.
-      induction l_l_a; simpl; intros; eauto.
-      intuition.
-      apply in_app_iff in H; intuition eauto.
-      apply IHl_l_a in H0; destruct H0; intuition eauto.
-    Qed.
-
-          Lemma NoDup_map_fst_dedup_by_fst:
-        forall A AEQ B (l:list (A * B)),
-          NoDup (map fst (dedup_by_fst AEQ l)).
-      Proof.
-        induction l; simpl; intros; eauto.
-        constructor.
-        destruct (in_dec AEQ (fst a) (map fst l)); eauto.
-        simpl; constructor; eauto.
-        intros Hx.
-        apply in_map_iff in Hx; cleanup.
-        apply in_dedup_by_fst in H0; eauto.
-        rewrite <- H in *.
-        apply n; apply in_map; eauto.
-      Qed.
-
-
-  Lemma list_upd_batch_eq_list_upd_batch_total:
-    forall A AEQ V l_a1 l_v1 l_a2 l_v2 (tm: @total_mem A AEQ V) m,
-      Mem.list_upd_batch m l_a1 l_v1 =
-      Mem.list_upd_batch m l_a2 l_v2 ->
-      Forall (Forall (fun a => m a = None)) l_a1 ->
-      Forall (Forall (fun a => m a = None)) l_a2 ->
-      Forall2 (fun l_a l_v => length l_a = length l_v) l_a1 l_v1 ->
-      Forall2 (fun l_a l_v => length l_a = length l_v) l_a2 l_v2 ->
-      list_upd_batch tm l_a1  l_v1 =
-      list_upd_batch tm l_a2 l_v2.
-  Proof.
-    intros.
-    do 2 rewrite list_upd_batch_to_upd_batch in *; eauto.
-    setoid_rewrite list_upd_batch_to_upd_batch_total; eauto.
-    setoid_rewrite upd_batch_dedup_by_fst_total.
-    eapply upd_batch_eq_upd_batch_total; eauto.            
-    repeat rewrite <- upd_batch_dedup_by_fst; eauto.
-    all: try solve [eapply flatten_length_eq; eauto].
-    apply Forall_forall; intros.
-    apply in_map_iff in H4; cleanup.
-    apply in_dedup_by_fst in H5.
-    destruct x0; simpl in *;
-    apply in_combine_l in H5.
-    apply in_flatten in H5; cleanup.
-    eapply Forall_forall in H0; eauto.
-    eapply Forall_forall in H0; eauto.
-
-    apply Forall_forall; intros.
-    apply in_map_iff in H4; cleanup.
-    apply in_dedup_by_fst in H5.
-    destruct x0; simpl in *;
-    apply in_combine_l in H5.
-    apply in_flatten in H5; cleanup.
-    eapply Forall_forall in H1; eauto.
-    eapply Forall_forall in H1; eauto.
-
-    apply NoDup_map_fst_dedup_by_fst.
-    apply NoDup_map_fst_dedup_by_fst. 
-  Qed.
-  
-  Lemma empty_mem_list_upd_batch_eq_list_upd_batch_total:
-    forall A AEQ V l_a1 l_v1 l_a2 l_v2 (tm: @total_mem A AEQ V),
-      Mem.list_upd_batch empty_mem l_a1 l_v1 =
-      Mem.list_upd_batch empty_mem l_a2 l_v2 ->
-      Forall2 (fun l_a l_v => length l_a = length l_v) l_a1 l_v1 ->
-      Forall2 (fun l_a l_v => length l_a = length l_v) l_a2 l_v2 ->
-      list_upd_batch tm l_a1  l_v1 =
-      list_upd_batch tm l_a2 l_v2.
-  Proof.
-    intros.
-    eapply list_upd_batch_eq_list_upd_batch_total; eauto.
-    eapply Forall_forall; intuition.
-    eapply Forall_forall; intuition.
-    eapply Forall_forall; intuition.
-    eapply Forall_forall; intuition.
-  Qed.
-
-
-  
-    Lemma upd_batch_in_some_total_mem :
-      forall A AEQ V l_a l_v (m: @mem A AEQ V) (tm: @total_mem A AEQ V) a v,
-        Mem.upd_batch m l_a l_v a = Some v ->
-        m a = None ->
-        NoDup l_a ->
-        upd_batch tm l_a l_v a = v.
-    Proof.
-      induction l_a; simpl; intros; try congruence.
-      destruct l_v; simpl; try congruence.
-      destruct (AEQ a a0); subst.
-      inversion H1; cleanup.
-      rewrite upd_batch_upd; eauto.
-      rewrite Mem.upd_batch_upd in H; eauto.
-      rewrite Mem.upd_eq in H; eauto.
-      rewrite upd_eq; eauto.
-      congruence.
-      eapply IHl_a; eauto.
-      rewrite Mem.upd_ne; eauto.
-      inversion H1; eauto.
-    Qed.
+(*** Lemmas ***)
 
     Lemma log_rep_forall2_txns_length_match:
     forall txns s,
@@ -750,7 +174,6 @@ Set Nested Proofs Allowed.
     rewrite firstn_length_l; eauto.
     repeat rewrite map_length; eauto.
   Qed.
-
 
 
 (*** SPECS ***)
@@ -1270,8 +693,7 @@ Proof.
         intros; simpl.
         eapply Forall_forall in H12; eauto.
         unfold txn_well_formed in H12; logic_clean.
-        eapply Forall_forall in H35; eauto; lia.
-        
+        eapply Forall_forall in H37; eauto; lia.        
       }
       setoid_rewrite A.
       rewrite shift_list_upd_batch_set_comm; eauto.
@@ -1336,8 +758,8 @@ Proof.
     
     unfold log_rep, log_rep_general, log_rep_explicit,
     log_rep_inner, txns_valid in *; cleanup; simpl in *. 
-    inversion H15; simpl in *; cleanup.
-    unfold txn_well_formed in H2; cleanup.
+    inversion H16; simpl in *; cleanup.
+    unfold txn_well_formed in H3; cleanup.
     rewrite firstn_app2; eauto.
     unfold log_header_block_rep in *; simpl in *; cleanup.
     simpl; intuition eauto.
@@ -1364,7 +786,7 @@ Proof.
         lia.
       }
       {
-        eapply H13; lia.
+        eapply H14; lia.
       }
       {
         unfold sumbool_agree; intros; intuition eauto.
@@ -1374,18 +796,18 @@ Proof.
       }
     }
     {
-      rewrite H13; simpl; eauto.
+      rewrite H14; simpl; eauto.
     }
     rewrite map_length; eauto.
     }
     {
-      rewrite app_length in H11.
+      rewrite app_length in H12.
       repeat cleanup_pairs.
       unfold log_rep, log_rep_general, log_rep_explicit,
       log_rep_inner, header_part_is_valid, txns_valid in *;
       simpl in *; cleanup; simpl in *. 
           
-      rewrite <- H12 in *; simpl in *.
+      rewrite <- H13 in *; simpl in *.
       lia.
     }
     {
@@ -1397,7 +819,7 @@ Proof.
     {
       rewrite firstn_app2; eauto.    
       apply Forall_forall; intros.
-      apply in_map_iff in H8; cleanup.
+      apply in_map_iff in H10; cleanup.
       eapply_fresh Forall_forall in f; eauto.
       pose proof data_fits_in_disk.
       split; try lia.
@@ -1956,7 +1378,7 @@ Proof.
                  rewrite upd_batch_to_list_upd_batch_singleton.
                  setoid_rewrite <- list_upd_batch_app at 2.
                  unfold log_rep_general, log_rep_explicit, log_rep_inner, txns_valid in *; logic_clean.
-                 rewrite <- H10.
+                 rewrite <- H11.
                  erewrite RepImplications.bimap_get_addr_list.
                  4: eauto.
                  rewrite list_upd_batch_firstn_noop; eauto.                 
@@ -1964,7 +1386,7 @@ Proof.
                  eauto.
                  rewrite map_length; eauto.
                  unfold log_rep_general, log_rep_explicit, log_rep_inner, txns_valid in *; logic_clean.
-                 rewrite <- H10.                 
+                 rewrite <- H11.                 
                  erewrite RepImplications.bimap_get_addr_list.
                  repeat rewrite firstn_length, map_length; eauto.
                  3: eauto.
@@ -1982,7 +1404,7 @@ Proof.
                  rewrite total_mem_map_fst_sync_noop.
                  rewrite total_mem_map_fst_list_upd_batch_set.
                  unfold log_rep_general, log_rep_explicit, log_rep_inner, txns_valid in *; logic_clean.
-                 rewrite <- H10.
+                 rewrite <- H11.
                  erewrite RepImplications.bimap_get_addr_list.
                  4: eauto.
                  rewrite TotalMem.list_upd_batch_noop; eauto.
@@ -2006,20 +1428,21 @@ Proof.
                  setoid_rewrite <- shift_upd_noop at 6.
                  rewrite upd_list_upd_batch_upd_noop.
                  setoid_rewrite shift_upd_noop.
-                 unfold log_rep_general, log_rep_explicit, log_rep_inner, txns_valid in *; simpl in *; logic_clean.
-                 rewrite <- H10.
+                 unfold log_rep_general, log_rep_explicit,
+                 log_rep_inner, txns_valid in *; simpl in *; logic_clean.
+                 rewrite <- H11.
                  erewrite RepImplications.bimap_get_addr_list.
                  4: eauto.
                  rewrite TotalMem.list_upd_batch_noop; eauto.
                  {
                    apply forall_forall2.
                    apply Forall_forall; intros.
-                   rewrite <- combine_map in H12.
-                   apply in_map_iff in H12; cleanup.
+                   rewrite <- combine_map in H13.
+                   apply in_map_iff in H13; cleanup.
                    simpl.
-                   eapply Forall_forall in H11; eauto.
-                   unfold txn_well_formed in H11; logic_clean.
-                   rewrite H14.
+                   eapply Forall_forall in H12; eauto.
+                   unfold txn_well_formed in H12; logic_clean.
+                   rewrite H15.
                    apply firstn_length_l; eauto.
                    lia.
                    repeat rewrite map_length; eauto.
@@ -2027,12 +1450,12 @@ Proof.
                  {
                    apply forall_forall2.
                    apply Forall_forall; intros.
-                   rewrite <- combine_map in H12.
-                   apply in_map_iff in H12; cleanup.
+                   rewrite <- combine_map in H13.
+                   apply in_map_iff in H13; cleanup.
                    simpl.
-                   eapply Forall_forall in H11; eauto.
-                   unfold txn_well_formed in H11; logic_clean.
-                   rewrite H14.
+                   eapply Forall_forall in H12; eauto.
+                   unfold txn_well_formed in H12; logic_clean.
+                   rewrite H15.
                    apply firstn_length_l; eauto.
                    lia.
                    repeat rewrite map_length; eauto.
@@ -2049,12 +1472,12 @@ Proof.
                    log_rep_inner, txns_valid in *; logic_clean.
                    apply forall_forall2.
                    apply Forall_forall; intros.
-                   rewrite <- combine_map in H12.
-                   apply in_map_iff in H12; cleanup.
+                   rewrite <- combine_map in H13.
+                   apply in_map_iff in H13; cleanup.
                    simpl.
-                   eapply Forall_forall in H11; eauto.
-                   unfold txn_well_formed in H11; logic_clean.
-                   rewrite H14.
+                   eapply Forall_forall in H12; eauto.
+                   unfold txn_well_formed in H12; logic_clean.
+                   rewrite H15.
                    apply firstn_length_l; eauto.
                    lia.
                    repeat rewrite map_length; eauto.
@@ -2151,7 +1574,7 @@ Proof.
                 lia.
               }
               intros; lia.
-              intros; apply H8; lia.
+              intros; apply H9; lia.
               {
                 unfold sumbool_agree; intros; intuition eauto.
                 destruct (addr_dec x3 y); subst.
@@ -2161,9 +1584,9 @@ Proof.
               {
                 unfold log_crash_rep in *; cleanup.
                 simpl in *.
-                unfold log_rep_inner, txns_valid in H16; cleanup.
-                inversion H19; cleanup.
-                unfold txn_well_formed in H22; simpl in *; cleanup.
+                unfold log_rep_inner, txns_valid in H17; cleanup.
+                inversion H20; cleanup.
+                unfold txn_well_formed in H23; simpl in *; cleanup.
                 rewrite firstn_app2; eauto.
                 rewrite map_length; eauto.
               }
@@ -2181,9 +1604,9 @@ Proof.
                   lia.
                 }
                 intros; lia.
-                intros; apply H8; lia.
+                intros; apply H9; lia.
               }
-              rewrite H8; simpl; eauto.
+              rewrite H9; simpl; eauto.
              }
             {
               right; intuition eauto.
@@ -2207,7 +1630,7 @@ Proof.
                 lia.
               }
               intros; lia.
-              intros; apply H8; lia.
+              intros; apply H9; lia.
               {
                 unfold sumbool_agree; intros; intuition eauto.
                 destruct (addr_dec x3 y); subst.
@@ -2217,15 +1640,15 @@ Proof.
               {
                 unfold log_rep, log_rep_general, log_rep_explicit in *; cleanup.
                 simpl in *.
-                unfold log_rep_inner, txns_valid in H13; cleanup.
-                inversion H4; cleanup.
-                unfold txn_well_formed in H27; simpl in *; cleanup.
+                unfold log_rep_inner, txns_valid in H14; cleanup.
+                inversion H6; cleanup.
+                unfold txn_well_formed in H28; simpl in *; cleanup.
                 rewrite firstn_app2; eauto.
                 rewrite map_length; eauto.
               }
-              rewrite H8; simpl; eauto.
+              rewrite H9; simpl; eauto.
             }
-            all: try rewrite H7, firstn_app2.
+            all: try rewrite H8, firstn_app2.
             all: try rewrite app_length;
             try rewrite map_length; try lia.
             {
@@ -2234,13 +1657,13 @@ Proof.
             }
             {
               apply Forall_forall; intros.
-              apply in_map_iff in H8; cleanup_no_match.
+              apply in_map_iff in H9; cleanup_no_match.
               eapply_fresh Forall_forall in f; eauto.
               pose proof data_fits_in_disk.
               split; try lia.
             }
             {
-              rewrite H7, app_length, map_length; lia.
+              rewrite H8, app_length, map_length; lia.
             }
           }
           unfold log_rep in *; logic_clean.
@@ -2280,7 +1703,7 @@ Proof.
                 lia.
               }
               intros; lia.
-              intros; apply H9; lia.
+              intros; apply H10; lia.
               {
                 unfold sumbool_agree; intros; intuition eauto.
                 destruct (addr_dec x2 y); subst.
@@ -2290,15 +1713,15 @@ Proof.
               {
                 unfold log_rep, log_rep_general, log_rep_explicit in *; cleanup.
                 simpl in *.
-                unfold log_rep_inner, txns_valid in H13; cleanup.
-                inversion H4; cleanup.
-                unfold txn_well_formed in H27; simpl in *; cleanup.
+                unfold log_rep_inner, txns_valid in H14; cleanup.
+                inversion H6; cleanup.
+                unfold txn_well_formed in H28; simpl in *; cleanup.
                 rewrite firstn_app2; eauto.
                 rewrite map_length; eauto.
               }
-              rewrite H9; simpl; eauto.
+              rewrite H10; simpl; eauto.
             }
-            all: try rewrite H7, firstn_app2.
+            all: try rewrite H8, firstn_app2.
             all: try rewrite app_length;
             try rewrite map_length; try lia.
             {
@@ -2307,13 +1730,13 @@ Proof.
             }
             {
               apply Forall_forall; intros.
-              apply in_map_iff in H8; cleanup_no_match.
+              apply in_map_iff in H9; cleanup_no_match.
               eapply_fresh Forall_forall in f; eauto.
               pose proof data_fits_in_disk.
               split; try lia.
             }
             {
-              rewrite H7, app_length, map_length; lia.
+              rewrite H8, app_length, map_length; lia.
             }
         }
         {(** write_batch_to_cache_crashed **)
@@ -2359,7 +1782,7 @@ Proof.
                 lia.
               }
               intros; lia.
-              intros; apply H10; lia.
+              intros; apply H11; lia.
               {
                 unfold sumbool_agree; intros; intuition eauto.
                 destruct (addr_dec x5 y); subst.
@@ -2369,15 +1792,15 @@ Proof.
               {
                 unfold log_rep, log_rep_general, log_rep_explicit in *; cleanup.
                 simpl in *.
-                unfold log_rep_inner, txns_valid in H13; cleanup.
+                unfold log_rep_inner, txns_valid in H14; cleanup.
                 inversion H1; cleanup.
-                unfold txn_well_formed in H27; simpl in *; cleanup.
+                unfold txn_well_formed in H28; simpl in *; cleanup.
                 rewrite firstn_app2; eauto.
                 rewrite map_length; eauto.
               }
-              rewrite H10; simpl; eauto.
+              rewrite H11; simpl; eauto.
             }
-            all: try rewrite H9, firstn_app2.
+            all: try rewrite H10, firstn_app2.
             all: try rewrite app_length;
             try rewrite map_length; try lia.
             {
@@ -2392,7 +1815,7 @@ Proof.
               split; try lia.
             }
             {
-              rewrite H9, app_length, map_length; lia.
+              rewrite H10, app_length, map_length; lia.
             }
         }
       }
